code/mpfr/MPFR.Add1sp1.fst
@@ -30,7 +30,7 @@ module U32 = FStar.UInt32
 (* intermediate results *)
 private type mpfr_tmp_exp_t = x:mpfr_exp_t{I64.(x >=^ mpfr_EMIN /\ x <=^ mpfr_EMAX +^ 1L)}
 
-private noeq type state = {
+noeq type state = {
     sh:mpfr_reg_prec_t;
     bx:mpfr_tmp_exp_t;
     rb:mp_limb_t;
@@ -209,35 +209,54 @@ inline_for_extraction val mpfr_add_one_ulp:
     mpfr_round2_cond (add_one_ulp (as_normal h0 a)) rnd_mode (as_fp h1 a) /\
     I32.v t = mpfr_add1sp1_add_one_ulp_ternary_spec (as_normal h0 a) rnd_mode))
 
-let mpfr_add_one_ulp a ap rnd_mode sh bx =admit();
+inline_for_extraction val mpfr_add_one_ulp_carry:
+    a:mpfr_ptr -> ap:buffer mp_limb_t -> rnd_mode:mpfr_rnd_t ->
+    sh:mpfr_reg_prec_t -> bx:mpfr_exp_t -> Stack i32
+    (requires (fun h -> 
+    mpfr_live h a /\ length (as_struct h a).mpfr_d = 1 /\ ap == (as_struct h a).mpfr_d /\
+    normal_cond h a /\ mpfr_PREC_COND (I64.v (as_struct h a).mpfr_prec) /\
+    sh = I64.(gmp_NUMB_BITS -^ (as_struct h a).mpfr_prec) /\
+    bx = (as_struct h a).mpfr_exp /\ mpfr_EXP_COND (I64.v bx) /\
+    (get h ap 0) +%^ (mpfr_LIMB_ONE <<^ (int64_to_uint32 sh)) =^ 0uL))
+    (ensures  (fun h0 t h1 -> 
+    mpfr_live h1 a /\ mpfr_modifies a h0 h1 /\ mpfr_valid_cond h1 a /\
+    mpfr_round2_cond (add_one_ulp (as_normal h0 a)) rnd_mode (as_fp h1 a) /\
+    I32.v t = mpfr_add1sp1_add_one_ulp_ternary_spec (as_normal h0 a) rnd_mode))
+
+let mpfr_add_one_ulp_carry a ap rnd_mode sh bx=
     let h0 = ST.get() in
     ap.(0ul) <- ap.(0ul) +%^ (mpfr_LIMB_ONE <<^ (int64_to_uint32 sh));
-    if ap.(0ul) =^ 0uL then begin
-        ap.(0ul) <- mpfr_LIMB_HIGHBIT;
-	let h1 = ST.get() in
-	lemma_reveal_modifies_1 ap h0 h1;
-	lemma_intro_modifies_2 a ap h0 h1;
-	if I64.(bx +^ 1L <=^ mpfr_EMAX) then begin
-	    mpfr_SET_EXP a I64.(bx +^ 1L);
-	    let h2 = ST.get() in
-	    lemma_pow2_mod 63 (I64.v sh);
-	    eval_abs_lt_intro_lemma (as_normal h0 a) (mpfr_max_value (as_normal h0 a).sign (as_normal h0 a).prec);
-	    eval_eq_intro_lemma (add_one_ulp (as_normal h0 a)) (as_normal h2 a);
-	     assert(mpfr_round2_cond (add_one_ulp (as_normal h0 a)) rnd_mode (as_fp h2 a));//
-	    mpfr_modifies_trans_lemma a h0 h1 h2;
-	    mpfr_RET (mpfr_SIGN a)
-	end else begin
-	    assert(eval_abs (as_normal h0 a) == mpfr_overflow_bound (I64.v (as_struct h0 a).mpfr_prec));
-	    let t = mpfr_overflow a rnd_mode (mpfr_SIGN a) in
-	    let h2 = ST.get() in
-	    mpfr_overflow_post_cond_lemma (add_one_ulp (as_normal h0 a)) (add_one_ulp (as_normal h0 a)).prec rnd_mode (I32.v t) (as_fp h2 a);
-	    mpfr_modifies_trans_lemma a h0 h1 h2;
-	    mpfr_RET t
-	end
-    end else begin
+    ap.(0ul) <- mpfr_LIMB_HIGHBIT;
+    let h1 = ST.get() in
+    lemma_reveal_modifies_1 ap h0 h1;
+    lemma_intro_modifies_2 a ap h0 h1;
+    if I64.(bx +^ 1L <=^ mpfr_EMAX) then begin
+       mpfr_SET_EXP a I64.(bx +^ 1L);
+	 let h2 = ST.get() in
+	 lemma_pow2_mod 63 (I64.v sh);
+	 eval_abs_lt_intro_lemma (as_normal h0 a) (mpfr_max_value (as_normal h0 a).sign (as_normal h0 a).prec);
+	 eval_eq_intro_lemma (add_one_ulp (as_normal h0 a)) (as_normal h2 a);
+	 assert(mpfr_round2_cond (add_one_ulp (as_normal h0 a)) rnd_mode (as_fp h2 a));//
+	 mpfr_modifies_trans_lemma a h0 h1 h2;
+	 mpfr_RET (mpfr_SIGN a)
+    end else begin 
+	assert(eval_abs (as_normal h0 a) == mpfr_overflow_bound (I64.v (as_struct h0 a).mpfr_prec));
+	let t = mpfr_overflow a rnd_mode (mpfr_SIGN a) in
+	let h2 = ST.get() in
+	mpfr_overflow_post_cond_lemma (add_one_ulp (as_normal h0 a)) (add_one_ulp (as_normal h0 a)).prec rnd_mode (I32.v t) (as_fp h2 a);
+	mpfr_modifies_trans_lemma a h0 h1 h2;
+	mpfr_RET t
+    end
+
+let mpfr_add_one_ulp a ap rnd_mode sh bx =
+    let h0 = ST.get() in
+    if ap.(0ul) +%^ (mpfr_LIMB_ONE <<^ (int64_to_uint32 sh)) =^ 0uL then
+        mpfr_add_one_ulp_carry a ap rnd_mode sh bx
+    else begin 
+        ap.(0ul) <- ap.(0ul) +%^ (mpfr_LIMB_ONE <<^ (int64_to_uint32 sh));
         let h1 = ST.get() in
 	lemma_pow2_multiple_le (v (get h0 ap 0)) 64 (I64.v sh);
-	 assert(v (get h0 ap 0) + pow2 (I64.v sh) = v (get h1 ap 0));//
+	assert(v (get h0 ap 0) + pow2 (I64.v sh) = v (get h1 ap 0));
 	lemma_pow2_mod (I64.v sh) (I64.v sh);
 	lemma_mod_distr_zero (v (get h0 ap 0)) (pow2 (I64.v sh)) (pow2 (I64.v sh));
         exp_impl_no_overflow_lemma (as_normal h1 a);
@@ -252,7 +271,7 @@ inline_for_extraction val mpfr_add1sp1_round:
         ap == (as_struct h a).mpfr_d /\
         (let high = {as_normal h a with exp = I64.v st.bx} in
         let p = high.prec in
-        as_val h (as_struct h a).mpfr_d * pow2 (high.len - 64) = high.limb /\
+        as_val h (as_struct h a).mpfr_d * pow2 high.len = high.limb * pow2 64 /\
         I64.v st.sh = I64.v gmp_NUMB_BITS - p /\
         mpfr_EXP_COND (I64.v st.bx))))
     (ensures  (fun h0 t h1 -> 
@@ -317,12 +336,12 @@ let mpfr_add1sp1 a b c rnd_mode p =
         let t = mpfr_overflow a rnd_mode (mpfr_SIGN a) in
 	let h2 = ST.get() in
 	mpfr_overflow_post_cond_lemma (add1sp_exact (as_reg_fp h0 b) (as_reg_fp h0 c)) (I64.v (as_struct h0 a).mpfr_prec) rnd_mode (I32.v t) (as_fp h2 a);
-	mpfr_modifies_trans_lemma a h0 h1 h2;
+//	mpfr_modifies_trans_lemma a h0 h1 h2;
 	t
     end else begin
         let t = mpfr_add1sp1_round a ap rnd_mode st in
 	let h2 = ST.get() in
 	mpfr_add1sp1_round_post_cond_lemma (add1sp_exact (as_reg_fp h0 b) (as_reg_fp h0 c)) (I64.v (as_struct h0 a).mpfr_prec) (as_normal_ h1 ({as_struct h1 a with mpfr_exp = st.bx})) (st.rb <> 0uL) (st.sb <> 0uL) rnd_mode (I32.v t) (as_fp h2 a);
-	mpfr_modifies_trans_lemma a h0 h1 h2;
+//	mpfr_modifies_trans_lemma a h0 h1 h2;
 	t
     end
