code/mpfr/MPFR.Sub1sp1.fst
@@ -5,6 +5,7 @@ open FStar.HyperStack
 open FStar.HyperStack.ST
 open FStar.Buffer
 open FStar.UInt64
+open FStar.UInt
 open FStar.Int.Cast
 open FStar.Mul
 open MPFR.Dyadic
@@ -18,6 +19,8 @@ open MPFR.Exceptions
 
 open MPFR.Exceptions.Lemma
 (*open MPFR.Sub1sp1.Lemma*)
+open MPFR.Add1sp1
+open MPFR.Add1sp1.Lemma
 
 module ST = FStar.HyperStack.ST
 module I32 = FStar.Int32
@@ -25,22 +28,6 @@ module I64 = FStar.Int64
 module U32 = FStar.UInt32
 
 #set-options "--z3refresh --z3rlimit 100 --max_fuel 1 --initial_fuel 0 --max_ifuel 1 --initial_ifuel 0"
-
-private type mpfr_tmp_exp_t = x:mpfr_exp_t{I64.(x >=^ mpfr_EMIN /\ x <=^ mpfr_EMAX +^ 1L)}
-
-private noeq type state = {
-    sh:mpfr_reg_prec_t;
-    bx:mpfr_tmp_exp_t;
-    rb:mp_limb_t;
-    sb:mp_limb_t
-}
-
-let mk_state sh bx rb sb = {
-    sh = sh;
-    bx = bx;
-    rb = rb;
-    sb = sb
-}
 
 let mpfr_sub1sp1_pre_cond h (a:mpfr_ptr) b c (p:mpfr_prec_t): GTot Type0=
         (* Memory safety *)
@@ -52,16 +39,16 @@ let mpfr_sub1sp1_pre_cond h (a:mpfr_ptr) b c (p:mpfr_prec_t): GTot Type0=
         (* Functional correctness *)
         I64.v p > 0 /\ I64.v p < 64 /\ p = (as_struct h a).mpfr_prec /\
         p = (as_struct h b).mpfr_prec /\ p = (as_struct h c).mpfr_prec /\
-        (as_struct h a).mpfr_sign = (as_struct h b).mpfr_sign /\
         mpfr_valid_cond h a /\ mpfr_reg_cond h b /\ mpfr_reg_cond h c
 
-let mpfr_sub1sp1_pre_cond_2 h (a:mpfr_ptr) b c bx cx ap bp cp: GTot Type0=
+let mpfr_sub1sp1_pre_cond_2 h (a:mpfr_ptr) b c bx cx ap bp cp p sh: GTot Type0=
  (as_struct h b).mpfr_exp=bx /\
  (as_struct h c).mpfr_exp=cx /\ 
- equal h (as_struct h a).mpfr_d h ap /\
- equal h (as_struct h b).mpfr_d h bp /\
- equal h (as_struct h c).mpfr_d h cp /\
- live h ap /\ live h bp /\ live h cp
+ (as_struct h a).mpfr_d==ap /\
+ (as_struct h b).mpfr_d==bp /\
+ (as_struct h c).mpfr_d==cp /\
+ live h ap /\ live h bp /\ live h cp /\
+ I64.v sh = I64.v gmp_NUMB_BITS - I64.v p
 
 let mpfr_sub1sp1_post_cond h0 t h1 (a:mpfr_ptr) b c (p:mpfr_reg_prec_t) rnd_mode exact: GTot Type0=
         (* Memory safety *)
@@ -73,27 +60,9 @@ let mpfr_sub1sp1_post_cond h0 t h1 (a:mpfr_ptr) b c (p:mpfr_reg_prec_t) rnd_mode
         mpfr_round_cond exact (I64.v p) rnd_mode (as_fp h1 a) /\
         mpfr_ternary_cond (I32.v t) exact (as_fp h1 a)
 
-let mpfr_sub1sp1_round_spec (high:normal_fp) (rb:bool) (sb:bool) (rnd_mode:mpfr_rnd_t):
-    Tot (r:normal_fp{r.prec = high.prec}) =
-    if rb = false && sb = false then high
-    else if MPFR_RNDN? rnd_mode then begin
-	if rb = false || (sb = false && is_even high)
-	then high
-	else add_one_ulp high
-    end else if mpfr_IS_LIKE_RNDZ rnd_mode (high.sign < 0) then high
-    else add_one_ulp high
-
-inline_for_extraction val count_leading_zeros: a:u64{not (a=^0uL)}->Tot (cnt:u32{U32.v cnt<32})
+inline_for_extraction val count_leading_zeros: a:u64{not (a=^0uL)}->Tot (cnt:u32{U32.v cnt<32 /\ v (a<<^cnt)>=pow2 63})
 
 let  count_leading_zeros a=admit()
-
-inline_for_extraction val mpfr_sub1sp1_round:(*Warning : the ensure part is too copy-pasted to be correct*)
-    a:mpfr_ptr -> ap:buffer mp_limb_t -> sh:mpfr_reg_prec_t -> bx:mpfr_reg_exp_t ->
-    rb:mp_limb_t -> sb:mp_limb_t -> rnd_mode:mpfr_rnd_t ->Stack i32
-    (requires (fun h->True))
-    (ensures (fun h0 r h1-> mpfr_live h1 a /\ mpfr_modifies a h0 h1 /\ mpfr_valid_cond h1 a /\ True))
-
-let mpfr_sub1sp1_round a ap bx rb sb rnd_mode=admit()
 
 inline_for_extraction val mpfr_sub1sp1_eq_branch_1:
     a:mpfr_ptr -> b:mpfr_ptr -> c:mpfr_ptr ->
@@ -102,7 +71,7 @@ inline_for_extraction val mpfr_sub1sp1_eq_branch_1:
     ->rnd_mode:mpfr_rnd_t->
     p:mpfr_reg_prec_t -> sh:mpfr_reg_prec_t -> Stack i32
     (requires (fun h->mpfr_sub1sp1_pre_cond h a b c p /\
-    mpfr_sub1sp1_pre_cond_2 h a b c bx cx ap bp cp /\
+    mpfr_sub1sp1_pre_cond_2 h a b c bx cx ap bp cp p sh /\
     I64.(bx=^cx) /\ as_val h bp=as_val h cp 
     ))
  (ensures (fun h0 t h1 -> 
@@ -114,51 +83,102 @@ let mpfr_sub1sp1_eq_branch_1 a b c ap bp cp bx cx rnd_mode p sh=
     mpfr_SET_ZERO a;
     mpfr_RET 0l
 
+val lemma_shift_left_mod_pow2: a:t -> s:U32.t -> k:nat -> Lemma
+  (requires ((v a)%(pow2 k)=0)/\U32.v s<64 /\ k<64)//could be proven without the k<64 condition
+  (ensures ((v (a<<^s))%(pow2 k)=0))
+  
+let lemma_shift_left_mod_pow2 a s k=
+   shift_left_value_lemma (v a) U32.(v s);//a<<^s=(a*2^s)%(2^64)
+   lemma_pow2_mod_mod (v a*pow2 U32.(v s)) 64 k;//a<<^s%(2^k)=a*(2^s)%(2^k)
+   lemma_mul_mod_zero (v a) (pow2 U32.(v s)) (pow2 k)
+
+let mpfr_sub1sp1_any_post_cond h0 s h1 (a:mpfr_ptr) b c (p:mpfr_reg_prec_t) rnd_mode exact: GTot Type0=
+        (* Memory safety *)
+        mpfr_live h1 a /\ mpfr_live h1 b /\ mpfr_live h1 c /\
+        length (as_struct h1 a).mpfr_d = 1 /\
+        length (as_struct h1 b).mpfr_d = 1 /\ length (as_struct h1 c).mpfr_d = 1 /\
+        modifies_1 (as_struct h1 a).mpfr_d h0 h1 /\ normal_cond h1 a /\ 
+        I64.(v ((as_struct h0 a).mpfr_prec)=v p) /\
+        I64.(v ((as_struct h0 b).mpfr_prec)=v p) /\
+        I64.(v ((as_struct h0 c).mpfr_prec)=v p) /\
+        mpfr_reg_cond h0 b /\ mpfr_reg_cond h0 c /\
+        (let r = sub1sp_exact (as_reg_fp h0 b) (as_reg_fp h0 c) in
+        normal_fp_cond r /\
+        mpfr_EXP_COND (I64.v s.bx) /\
+        as_val h1 (as_struct h1 a).mpfr_d * pow2 (r.len) = (high_mant r (I64.v p)).limb * (pow2 64) /\
+        I64.v s.sh = I64.v gmp_NUMB_BITS - I64.v p /\
+        I64.v s.bx = (high_mant r (I64.v p)).exp /\
+        (rb_def r (I64.v p) = (v s.rb <> 0)) /\
+        (sb_def r (I64.v p) = (v s.sb <> 0)) /\
+        (high_mant r (I64.v p)).sign = (as_normal h1 a).sign)
+        
 inline_for_extraction val mpfr_sub1sp1_eq:
     a:mpfr_ptr -> b:mpfr_ptr -> c:mpfr_ptr ->
     ap:buffer mp_limb_t -> bp:buffer mp_limb_t -> cp:buffer mp_limb_t ->
     bx:mpfr_reg_exp_t ->cx:mpfr_reg_exp_t
     ->rnd_mode:mpfr_rnd_t->
-    p:mpfr_reg_prec_t -> sh:mpfr_reg_prec_t -> Stack i32
+    p:mpfr_reg_prec_t -> sh:mpfr_reg_prec_t -> Stack state
     (requires (fun h-> mpfr_sub1sp1_pre_cond h a b c p /\
-    mpfr_sub1sp1_pre_cond_2 h a b c bx cx ap bp cp /\
-    I64.(bx=^cx)
+    mpfr_sub1sp1_pre_cond_2 h a b c bx cx ap bp cp p sh /\
+    I64.(bx=^cx) /\
+    I64.(as_val h bp<>as_val h cp)
     ))
     (ensures (fun h0 t h1->
-    let exact=sub1sp_exact (as_fp h0 b) (as_fp h0 c) in 
-    mpfr_sub1sp1_post_cond h0 t h1 a b c p rnd_mode exact))
+    let exact=sub1sp_exact (as_fp h0 b) (as_fp h0 c) in
+    mpfr_sub1sp1_any_post_cond h0 t h1 a b c p rnd_mode exact))
 
-let mpfr_sub1sp1_eq a b c ap bp cp bx cx rnd_mode p sh =
-    if (bp.(0ul)=cp.(0ul)) then mpfr_sub1sp1_eq_branch_1 a b c ap bp cp bx cx rnd_mode p sh
-    else begin admit();
-       if(cp.(0ul)>^bp.(0ul)) then begin
-         //mpfr_SET_OPPOSITE_SIGN a b;
-         let a0=cp.(0ul) -^ bp.(0ul) in
-         let cnt=count_leading_zeros a0 in
-         ap.(0ul) <- a0<<^cnt;
-         mpfr_sub1sp1_round a ap bx 0uL 0uL rnd_mode
-       end else begin 
-         //mpfr_SET_SAME_SIGN a b;
-         let a0=bp.(0ul) -^ cp.(0ul) in
-         let cnt=count_leading_zeros a0 in
-         ap.(0ul) <- a0<<^cnt;
-         mpfr_sub1sp1_round a ap bx 0uL 0uL rnd_mode
-       end
-    end
+let mpfr_sub1sp1_eq a b c ap bp cp bx cx rnd_mode p sh =admit();
+    let h0=ST.get() in
+    let vb= v bp.(0ul) in
+    let vc= v cp.(0ul) in
+    let vsh= I64.(v sh) in
+      if(cp.(0ul)>^bp.(0ul)) then begin
+        let a0=cp.(0ul) -^ bp.(0ul) in
+        let cnt=count_leading_zeros a0 in
+        mpfr_SET_OPPOSITE_SIGN a b;
+        ap.(0ul) <- a0<<^cnt;
+        lemma_mod_distr_sub_zero vc vb (pow2 vsh);
+        lemma_shift_left_mod_pow2 a0 cnt vsh;
+        let h1=ST.get() in
+        mk_state sh bx 0uL 0uL
+      end else begin 
+        let a0=bp.(0ul) -^ cp.(0ul) in
+        let cnt=count_leading_zeros a0 in
+        mpfr_SET_SAME_SIGN a b;
+        ap.(0ul) <- a0<<^cnt;
+        lemma_mod_distr_sub_zero vb vc (pow2 vsh);
+        lemma_shift_left_mod_pow2 a0 cnt vsh;
+        mk_state sh bx 0uL 0uL
+      end
 
 inline_for_extraction val mpfr_sub1sp1_gt:
     a:mpfr_ptr -> b:mpfr_ptr -> c:mpfr_ptr ->
     ap:buffer mp_limb_t -> bp:buffer mp_limb_t -> cp:buffer mp_limb_t ->
     bx:mpfr_reg_exp_t ->cx:mpfr_reg_exp_t
     ->rnd_mode:mpfr_rnd_t->
-    p:mpfr_reg_prec_t -> sh:mpfr_reg_prec_t -> Stack i32
-    (requires (fun h-> mpfr_live h a /\ mpfr_live h b /\ mpfr_live h c /\ length ap>0 /\ length bp>0 /\ length cp>0 /\ live h ap /\ live h bp /\ live h cp /\ I64.v sh = I64.v gmp_NUMB_BITS - I64.v p))
-    (ensures (fun h s h1->True))
+    p:mpfr_reg_prec_t -> sh:mpfr_reg_prec_t -> Stack state
+    (requires (fun h->
+    mpfr_sub1sp1_pre_cond h a b c p /\
+    mpfr_sub1sp1_pre_cond_2 h a b c bx cx ap bp cp p sh /\
+    I64.(bx >^ cx)))
+    (ensures (fun h0 t h1->
+    let exact=sub1sp_exact (as_fp h0 b) (as_fp h0 c) in
+    mpfr_sub1sp1_any_post_cond h0 t h1 a b c p rnd_mode exact))
 
-let mpfr_sub1sp1_gt a b c ap bp cp bx cx rnd_mode p sh =
+let mpfr_sub1sp1_gt a b c ap bp cp bx cx rnd_mode p sh =admit()(*;
     let d = I64.(bx-^cx) in
     let mask = mpfr_LIMB_MASK (int64_to_uint32 sh) in
-    admit()
+    if I64.(d <^ gmp_NUMB_BITS) then begin
+      let sb=0uL -^ (cp.(0ul) <<^ (int64_to_uint32 I64.(gmp_NUMB_BITS -^ d))) in
+      let a0_tmp = bp.(0ul) -^ (if v sb=0 then 0uL else 1uL) -^ (cp.(0ul)>>^(int64_to_uint32 d)) in
+      assert(v a0_tmp>0);
+      let cnt=count_leading_zeros a0_tmp in
+      let a0=if U32.(v cnt)>0 then (a0_tmp<<^cnt) |^ (sb>>^U32.(int64_to_uint32 gmp_NUMB_BITS -^ cnt)) else a0_tmp in
+      ap.(0ul)<-a0 &^ (lognot mask);
+      mpfr_sub1sp1_round a ap sh bx 0uL 0uL rnd_mode
+    end
+    else mpfr_RET 0l
+*)
 
 (* specifications for mpfr_sub1sp1 *)
 val mpfr_sub1sp1: a:mpfr_ptr -> b:mpfr_ptr -> c:mpfr_ptr ->
@@ -167,6 +187,21 @@ val mpfr_sub1sp1: a:mpfr_ptr -> b:mpfr_ptr -> c:mpfr_ptr ->
     (ensures  (fun h0 t h1 ->
     let exact=sub1sp_exact (as_fp h0 b) (as_fp h0 c) in
     mpfr_sub1sp1_post_cond h0 t h1 a b c p rnd_mode exact))
+val mpfr_add1sp1_round_post_cond_lemma: a:normal_fp{mpfr_EXP_COND a.exp} ->
+    p:pos{mpfr_PREC_COND p} ->
+    high:normal_fp{high.prec = p /\ high.sign = (high_mant a p).sign  /\
+                   high.exp = (high_mant a p).exp /\
+		   high.limb * pow2 a.len = (high_mant a p).limb * pow2 high.len} ->
+    rb:bool{rb = rb_def a p} -> sb:bool{sb = sb_def a p} -> rnd_mode:mpfr_rnd_t ->
+    t:int -> r:mpfr_fp{r.prec = p} -> Lemma
+    (requires (mpfr_round2_cond (mpfr_add1sp1_round_spec high rb sb rnd_mode) rnd_mode r /\
+               t = mpfr_add1sp1_ternary_spec high rb sb rnd_mode))
+    (ensures  (mpfr_round_cond a p rnd_mode r /\
+               mpfr_ternary_cond t a r))
+
+let mpfr_add1sp1_round_post_cond_lemma a p high rb sb rnd_mode t r =admit();
+    mpfr_round_cond_lemma a p high rb sb rnd_mode r;
+    mpfr_ternary_cond_lemma a p high rb sb rnd_mode t r
 
 let mpfr_sub1sp1 a b c rnd_mode p =
     let bx=mpfr_GET_EXP b in
@@ -175,28 +210,40 @@ let mpfr_sub1sp1 a b c rnd_mode p =
     let bp=mpfr_MANT b in
     let cp=mpfr_MANT c in
     let sh=I64.(gmp_NUMB_BITS -^ p) in
-    if I64.(bx =^ cx) then mpfr_sub1sp1_eq a b c ap bp cp bx cx rnd_mode p sh else begin admit();
-   let bx,cx,bp,cp=(if I64.(bx >=^ cx) then (mpfr_SET_SAME_SIGN a b;bx,cx,bp,cp) else (mpfr_SET_OPPOSITE_SIGN a b;cx,bx,cp,bp)) in
-    ignore (mpfr_sub1sp1_gt a b c ap bp cp bx cx rnd_mode p sh);0l
-    end
-  (*  let st = mpfr_sub1sp1_any a b c ap p in()*)
-   (* let h1 = ST.get() in
-    lemma_reveal_modifies_1 (mpfr_MANT a) h0 h1;
-    lemma_intro_modifies_2 a (mpfr_MANT a) h0 h1;
-    if I64.(st.bx >^ mpfr_EMAX) then begin
+    let bp0ul=bp.(0ul) in
+    let cp0ul=cp.(0ul) in
+    let h0=ST.get() in
+    if I64.(bx =^ cx) && (bp0ul=cp0ul) then
+       mpfr_sub1sp1_eq_branch_1 a b c ap bp cp bx cx rnd_mode p sh
+    else begin
+    let st=if I64.(bx =^ cx) then begin
+      mpfr_sub1sp1_eq a b c ap bp cp bx cx rnd_mode p sh
+    end else begin  admit();
+   let b,c,bx,cx,bp,cp=(if I64.(bx >=^ cx) then (mpfr_SET_SAME_SIGN a b;b,c,bx,cx,bp,cp) else (mpfr_SET_OPPOSITE_SIGN a b;c,b,cx,bx,cp,bp)) in       
+    mpfr_sub1sp1_gt a b c ap bp cp bx cx rnd_mode p sh
+    end in 
+    let h1 = ST.get() in
+    if I64.(st.bx <^ mpfr_EMIN) then begin
         let s = mpfr_SIGN a in
-        let t = mpfr_overflow a rnd_mode (mpfr_SIGN a) in
+        let t = mpfr_underflow a rnd_mode (mpfr_SIGN a) in
 	let h2 = ST.get() in
-	mpfr_overflow_post_cond_lemma (add1sp_exact (as_reg_fp h0 b) (as_reg_fp h0 c)) (I64.v (as_struct h0 a).mpfr_prec) rnd_mode (I32.v t) (as_fp h2 a);
-	mpfr_modifies_trans_lemma a h0 h1 h2;
+	mpfr_underflow_post_cond_lemma (sub1sp_exact (as_reg_fp h0 b) (as_reg_fp h0 c)) (I64.v (as_struct h0 a).mpfr_prec) rnd_mode (I32.v t) (as_fp h2 a);
 	t
-    end else begin
+    end else begin (*Rounding is the same as for add1sp1 (modulo an optimization), so this is copied from mpfr_add1sp1*)
         let t = mpfr_add1sp1_round a ap rnd_mode st in
 	let h2 = ST.get() in
-	mpfr_add1sp1_round_post_cond_lemma (add1sp_exact (as_reg_fp h0 b) (as_reg_fp h0 c)) (I64.v (as_struct h0 a).mpfr_prec) (as_normal_ h1 ({as_struct h1 a with mpfr_exp = st.bx})) (st.rb <> 0uL) (st.sb <> 0uL) rnd_mode (I32.v t) (as_fp h2 a);
-	mpfr_modifies_trans_lemma a h0 h1 h2;
+	mpfr_add1sp1_round_post_cond_lemma (sub1sp_exact (as_reg_fp h0 b) (as_reg_fp h0 c)) (I64.v (as_struct h0 a).mpfr_prec) (as_normal_ h1 ({as_struct h1 a with mpfr_exp = st.bx})) (st.rb <> 0uL) (st.sb <> 0uL) rnd_mode (I32.v t) (as_fp h2 a);
 	t
     end
+   end
 
-On fait l'arrondi
+(*
+   (let r = sub1sp_exact (as_reg_fp h0 b) (as_reg_fp h0 c) in
+        normal_fp_cond r /\
+        mpfr_EXP_COND (I64.v s.bx) /\
+        as_val h1 (as_struct h1 a).mpfr_d * pow2 (r.len) = (high_mant r (I64.v p)).limb * (pow2 64) /\
+        I64.v s.sh = I64.v gmp_NUMB_BITS - I64.v p /\
+        I64.v s.bx = (high_mant r (I64.v p)).exp /\
+        (rb_def r (I64.v p) = (v s.rb <> 0)) /\
+        (sb_def r (I64.v p) = (v s.sb <> 0)))
 *)
